Split extensions.v into two files: 1) extension.v contains interfaces 2) extension_proof.v contains just proofs
The specification of "compilable" extensions is still in extension_proof.v 
since it's liable to change pretty soon.

Also: add to the Makefile seplog_extension.v, which defines a Hoare logic 
rule for verification w/r/t extensions

veric/extension_proof.v
@@ -1,217 +1,20 @@
 Load loadpath.
 Require Import msl.predicates_hered.
-Require Import veric.sim veric.step_lemmas veric.base veric.expr veric.extspec 
-               veric.juicy_extspec.
-Require Import ListSet.
+Require Import veric.sim veric.step_lemmas veric.base veric.expr 
+               veric.extspec veric.juicy_extspec veric.extension.
 
 Set Implicit Arguments.
 
-Lemma extfunct_eqdec : forall ef1 ef2 : AST.external_function, 
-  {ef1=ef2} + {~ef1=ef2}.
-Proof. intros ef1 ef2; repeat decide equality; apply Address.EqDec_int. Qed.
-
-Definition is_true (b: bool) := b=true.
-Local Coercion is_true: bool >-> Sortclass.
-
-Notation IN := (ListSet.set_mem extfunct_eqdec).
-Notation NOTIN := (fun ef l => ListSet.set_mem extfunct_eqdec ef l = false).
-Notation DIFF := (ListSet.set_diff extfunct_eqdec).
-
-Lemma in_diff (ef: AST.external_function) (l r: list AST.external_function) :
-  IN ef l -> NOTIN ef r -> IN ef (DIFF l r).
-Proof.
-simpl; intros H1 H2; apply set_mem_correct2. 
-apply set_mem_correct1 in H1.
-apply set_mem_complete1 in H2.
-apply set_diff_intro; auto.
-Qed.
-
-(*linking external specification "sigma" with an extension implementing
-   functions in "handled" corresponds to removing the functions in handled from
-   the external specification*)
-
-Definition link_ext_spec (M Z: Type) (handled: list AST.external_function) 
-  (sigma: external_specification M AST.external_function Z) :=
-  Build_external_specification M AST.external_function Z
-    (ext_spec_type sigma)
-    (fun (ef: AST.external_function) (x: ext_spec_type sigma ef)
-         (tys: list typ) (args: list val) (z: Z) (m: M) => 
-             if ListSet.set_mem extfunct_eqdec ef handled then False 
-             else ext_spec_pre sigma ef x tys args z m)
-    (fun (ef: AST.external_function) (x: ext_spec_type sigma ef)
-         (ty: option typ) (ret: option val) (z: Z) (m: M) => 
-             if ListSet.set_mem extfunct_eqdec ef handled then True
-             else ext_spec_post sigma ef x ty ret z m).
-
-Program Definition link_juicy_ext_spec (Z: Type) (handled: list AST.external_function)
-  (sigma: juicy_ext_spec Z) :=
-  Build_juicy_ext_spec Z (link_ext_spec handled sigma) _ _.
-Next Obligation.
-if_tac; [unfold hereditary; auto|].
-generalize JE_pre_hered; unfold hereditary; intros; eapply H; eauto.
-Qed.
-Next Obligation.
-if_tac; [unfold hereditary; auto|].
-generalize JE_post_hered; unfold hereditary; intros; eapply H; eauto.
-Qed.
-
-(*an external signature "ext_sig" is a list of handled functions together with
-   an external specification*)
-
-Section ExtSig.
-Variables M Z: Type.
-
-Inductive ext_sig := 
-  mkextsig: forall (functs: list AST.external_function)
-                   (extspec: external_specification M external_function Z), 
-    ext_sig.
-
-Definition extsig2functs (sigma: ext_sig) := 
-  match sigma with mkextsig l _ => l end.
-Coercion extsig2functs : ext_sig >-> list.
-
-Definition extsig2extspec (sigma: ext_sig) :=
-  match sigma with mkextsig functs spec => spec end.
-Coercion extsig2extspec : ext_sig >-> external_specification.
-
-Definition spec_of (ef: AST.external_function) (sigma: ext_sig) :=
-  (ext_spec_pre sigma ef, ext_spec_post sigma ef).
-
-End ExtSig.
-
-Record juicy_ext_sig (Z: Type): Type := mkjuicyextsig {
-  JE_functs:> list external_function;
-  JE_extspec:> juicy_ext_spec Z
-}.
-
-Definition juicy_extsig2extsig (Z: Type) (je: juicy_ext_sig Z) :=
-  mkextsig (JE_functs je) (JE_extspec je).
-Coercion juicy_extsig2extsig: juicy_ext_sig >-> ext_sig.
-
-Definition link (T Z: Type) (esig: ext_sig T Z) 
-      (handled: list AST.external_function) :=
-  mkextsig handled (link_ext_spec handled esig).
-
-Definition juicy_link (Z: Type) (jesig: juicy_ext_sig Z) 
-      (handled: list AST.external_function) :=
-  mkjuicyextsig handled (link_juicy_ext_spec handled jesig).
-
-(*ef:{P}{Q} (ext_sig spec) is a subtype of ef:{P'}{Q'} (spec. assumed by client)*)
-Definition linkable (M Z Zext: Type) (proj_zext: Z -> Zext)
-      (handled: list AST.external_function) 
-      (client_sig: ext_sig M Z) (ext_sig: ext_sig M Zext) := 
-  forall ef P Q P' Q', 
-    IN ef (DIFF client_sig handled) -> 
-    spec_of ef ext_sig = (P, Q) -> 
-    spec_of ef client_sig = (P', Q') -> 
-    forall x' tys args m z, P' x' tys args z m -> 
-      exists x, P x tys args (proj_zext z) m /\
-      forall ty ret m' z', Q x ty ret (proj_zext z') m' -> Q' x' ty ret z' m'.
-
-Module Extension. 
-Record Sig
-  (G: Type) (*global environments*)
-  (xT: Type) (*corestates of extended semantics*)
-  (cT: nat -> Type) (*corestates of core semantics*)
-  (M: Type) (*memories*)
-  (D: Type) (*initialization data*)
-  (Z: Type) (*external states*)
-  (Zint: Type) (*portion of Z implemented by extension*)
-  (Zext: Type) (*portion of Z external to extension*)
-
-  (esem: CoreSemantics G xT M D) (*extended semantics*)
-  (csem: forall i:nat, option (CoreSemantics G (cT i) M D)) (*a set of core semantics*)
-
-  (client_sig: ext_sig M Z) 
-  (esig: ext_sig M Zext)
-  (handled: list AST.external_function) := Make {
-
-    (*generalized projection of core i from state s*)
-    proj_core : forall i:nat, xT -> option (cT i);
-    core_exists : forall ge i s c' m s' m', 
-      corestep esem ge s m s' m' -> proj_core i s' = Some c' -> 
-      exists c, proj_core i s = Some c;
-
-    (*the active (i.e., currently scheduled) core*)
-    active : xT -> nat;
-    active_csem : forall s, exists CS, csem (active s) = Some CS;
-    active_proj_core : forall s, exists c, proj_core (active s) s = Some c;
-
-    (*runnable=true when active s is runnable (i.e., not blocked
-      waiting on an external function call and not safely halted)*)
-    runnable : G -> xT -> bool;
-    runnable_false : forall ge s c CS,
-      runnable ge s = false -> 
-      csem (active s) = Some CS -> proj_core (active s) s = Some c -> 
-      (exists rv, safely_halted CS ge c = Some rv) \/
-      (exists ef, exists sig, exists args, at_external CS c = Some (ef, sig, args));
-
-    (*a core is no longer "at external" once the extension has returned 
-      to it with the result of the call on which it was blocked*)
-    after_at_external_excl : forall i CS c c' ret,
-      csem i = Some CS -> after_external CS ret c = Some c' -> 
-      at_external CS c' = None;
-
-    at_external_client_sig: forall s i CS c ef args sig,
-      csem i = Some CS -> proj_core i s = Some c -> 
-      at_external CS c = Some (ef, sig, args) -> 
-      IN ef client_sig;
-    notat_external_handled: forall s i CS c ef args sig,
-      csem i = Some CS -> proj_core i s = Some c -> 
-      at_external CS c = Some (ef, sig, args) -> 
-      at_external esem s = None -> 
-      IN ef handled;
-    at_external_not_handled: forall s ef args sig,
-      at_external esem s = Some (ef, sig, args) -> 
-      NOTIN ef handled;
-
-    (*type xT embeds Zint*)
-    proj_zint: xT -> Zint;
-    proj_zext: Z -> Zext;
-    zmult: Zint -> Zext -> Z;
-    zmult_proj: forall zint zext, proj_zext (zmult zint zext) = zext;
-    (*implemented "external" state is unchanged after truly external calls*)
-    ext_upd_at_external : forall ef sig args ret s s',
-      at_external esem s = Some (ef, sig, args) -> 
-      after_external esem ret s = Some s' -> 
-      proj_zint s = proj_zint s';
-
-    (*csem and esem are signature linkable*)
-    esem_csem_linkable: linkable proj_zext handled client_sig esig;
-
-    (*a global invariant characterizing "safe" extensions*)
-    all_safe (ge: G) (n: nat) (z: Z) (w: xT) (m: M) :=
-      forall i CS c, csem i = Some CS -> proj_core i w = Some c -> 
-        safeN CS client_sig ge n z c m
-}.
-
-End Extension. 
-
-Implicit Arguments Extension.Make [G xT cT M D Z Zint Zext].
-
-(*an extension E is safe when all states satisfy the "all_safe" invariant*)
-
-Section SafeExtension.
-Variables (G T M D Z Zint Zext: Type) (cT: nat -> Type)
-  (esem: CoreSemantics G T M D) (csem: forall i: nat, option (CoreSemantics G (cT i) M D))
-  (client_sig: ext_sig M Z) (esig: ext_sig M Zext) (handled: list AST.external_function).
-
-Import Extension.
-
-Definition safe_extension (E: Extension.Sig cT Zint esem csem client_sig esig handled) :=
-  forall ge n s m z, 
-    E.(all_safe) ge n (zmult E (proj_zint E s) z) s m -> 
-    safeN esem (link esig handled) ge n z s m.
-
-End SafeExtension.
-
 Section SafetyMonotonicity.
-Variables (G cT M D Zext: Type) (CS: CoreSemantics G cT M D)
-  (client_sig: ext_sig M Z) (handled: ext_sig M Zext).
+ Variables 
+  (G cT M D Zext: Type) 
+  (CS: CoreSemantics G cT M D)
+  (csig: ext_sig M Z) 
+  (handled: ext_sig M Zext).
 
 Lemma safety_monotonicity : forall ge n z c m,
-  safeN CS (link client_sig handled) ge n z c m -> 
-  safeN CS client_sig ge n z c m.
+  safeN CS (link csig handled) ge n z c m -> 
+  safeN CS csig ge n z c m.
 Proof. 
 intros ge n; induction n; auto.
 intros  ora c m; simpl; intros H1.
@@ -232,30 +35,43 @@ Qed.
 
 End SafetyMonotonicity.
 
-Section SafetyCriteria.
-Variables
-  (G xT M D Z Zint Zext: Type) (cT: nat -> Type)
-  (esem: CoreSemantics G xT M D) 
-  (csem: forall i:nat, option (CoreSemantics G (cT i) M D))
-  (client_sig: ext_sig M Z)
-  (esig: ext_sig M Zext)
-  (handled: list AST.external_function)
-  (E: Extension.Sig cT Zint esem csem client_sig esig handled).
+Module ExtensionSoundness. Section ExtensionSoundness.
+ Variables
+  (G: Type) (** global environments *)
+  (xT: Type) (** corestates of extended semantics *)
+  (cT: nat -> Type) (** corestates of core semantics *)
+  (M: Type) (** memories *)
+  (D: Type) (** initialization data *)
+  (Z: Type) (** external states *)
+  (Zint: Type) (** portion of Z implemented by extension *)
+  (Zext: Type) (** portion of Z external to extension *)
 
-Definition proj_zint := E.(Extension.proj_zint). 
-Local Coercion proj_zint : xT >-> Zint.
+  (esem: CoreSemantics G xT M D) (** extended semantics *)
+  (csem: forall i:nat, option (CoreSemantics G (cT i) M D)) (** a set of core semantics *)
 
-Definition proj_zext := E.(Extension.proj_zext).
-Local Coercion proj_zext : Z >-> Zext.
+  (csig: ext_sig M Z) (** client signature *)
+  (esig: ext_sig M Zext) (** extension signature *)
+  (handled: list AST.external_function) (** functions handled by this extension *)
+  (E: Extension.Sig cT Zint esem csem csig esig handled). 
 
-Notation ALL_SAFE := E.(Extension.all_safe).
+Import SafetyInterpolant.
+Import TruePropCoercion.
+
+Definition proj_zint := (proj_zint E). 
+Coercion proj_zint : xT >-> Zint.
+
+Definition proj_zext := (proj_zext E).
+Coercion proj_zext : Z >-> Zext.
+
+Notation ALL_SAFE := (all_safe E).
 Notation PROJ_CORE := E.(Extension.proj_core).
-Notation "zint \o zext" := (E.(Extension.zmult) zint zext) (at level 66, left associativity). 
+Notation "zint \o zext" := (E.(Extension.zmult) zint zext) 
+  (at level 66, left associativity). 
 Notation ACTIVE := (E.(Extension.active)).
 Notation RUNNABLE := (E.(Extension.runnable)).
 Notation "'CORE' i 'is' ( CS , c ) 'in' s" := 
   (csem i = Some CS /\ PROJ_CORE i s = Some c)
-  (at level 66, no associativity, only parsing).
+  (at level 66, no associativity).
 Notation core_exists := E.(Extension.core_exists).
 Notation active_csem := E.(Extension.active_csem).
 Notation active_proj_core := E.(Extension.active_proj_core).
@@ -265,121 +81,9 @@ Notation at_external_not_handled := E.(Extension.at_external_not_handled).
 Notation ext_upd_at_external := E.(Extension.ext_upd_at_external).
 Notation runnable_false := E.(Extension.runnable_false).
 
-Lemma all_safe_downward ge n z s m :
-  ALL_SAFE ge (S n) z s m -> ALL_SAFE ge n z s m.
-Proof. intros INV i CS c H2 H3; eapply safe_downward1; eauto. Qed.
-
-Inductive safety_criteria: Type := SafetyCriteria: forall 
-  (*coresteps preserve the invariant*)
-  (core_pres: forall ge n z (s: xT) c m CS s' c' m', 
-    ALL_SAFE ge (S n) (s \o z) s m -> 
-    CORE (ACTIVE s) is (CS, c) in s -> 
-    corestep CS ge c m c' m' -> corestep esem ge s m s' m' -> 
-    ALL_SAFE ge n (s' \o z) s' m')
-
-  (*corestates satisfying the invariant can corestep*)
-  (core_prog: forall ge n z s m c CS, 
-    ALL_SAFE ge (S n) z s m -> 
-    RUNNABLE ge s=true -> CORE (ACTIVE s) is (CS, c) in s -> 
-    exists c', exists s', exists m', 
-      corestep CS ge c m c' m' /\ corestep esem ge s m s' m' /\
-      CORE (ACTIVE s) is (CS, c') in s')
-
-  (*"handled" steps respect function specifications*)
-  (handled_pres: forall ge s z m (c: cT (ACTIVE s)) s' m' (c': cT (ACTIVE s)) 
-      (CS: CoreSemantics G (cT (ACTIVE s)) M D) ef sig args P Q x, 
-    let i := ACTIVE s in CORE i is (CS, c) in s -> 
-    at_external CS c = Some (ef, sig, args) -> 
-    ListSet.set_mem extfunct_eqdec ef handled = true -> 
-    spec_of ef client_sig = (P, Q) -> 
-    P x (sig_args sig) args (s \o z) m -> 
-    corestep esem ge s m s' m' -> 
-    CORE i is (CS, c') in s' -> 
-      ((at_external CS c' = Some (ef, sig, args) /\ P x (sig_args sig) args (s' \o z) m' /\
-        (forall j, ACTIVE s' = j -> i <> j)) \/
-      (exists ret, after_external CS ret c = Some c' /\ Q x (sig_res sig) ret (s' \o z) m')))
-
-  (*"handled" states satisfying the invariant can step or are safely halted;
-     core states that remain "at_external" over handled steps are unchanged*)
-
-  (handled_prog: forall ge n (z: Zext) (s: xT) m,
-    ALL_SAFE ge (S n) (s \o z) s m -> 
-    RUNNABLE ge s=false -> 
-    at_external esem s = None -> 
-    (exists s', exists m', corestep esem ge s m s' m' /\ 
-      forall i c CS, CORE i is (CS, c) in s -> 
-        exists c', CORE i is (CS, c') in s' /\ 
-          (forall ef args ef' args', 
-            at_external CS c = Some (ef, args) -> 
-            at_external CS c' = Some (ef', args') -> c=c')) \/
-    (exists rv, safely_halted esem ge s = Some rv))
-
-  (*safely halted threads remain halted*)
-  (safely_halted_halted: forall ge s m s' m' i CS c rv,
-    CORE i is (CS, c) in s -> 
-    safely_halted CS ge c = Some rv -> 
-    corestep esem ge s m s' m' -> 
-    CORE i is (CS, c) in s')
-
-  (*safety of other threads is preserved when handling one step of blocked
-     thread i*)
- 
-  (handled_rest: forall ge s m s' m' c CS,
-    CORE (ACTIVE s) is (CS, c) in s -> 
-    ((exists ef, exists sig, exists args, at_external CS c = Some (ef, sig, args)) \/ 
-      exists rv, safely_halted CS ge c = Some rv) -> 
-    at_external esem s = None -> 
-    corestep esem ge s m s' m' -> 
-    (forall j (CS0: CoreSemantics G (cT j) M D) c0, ACTIVE s <> j ->  
-      (CORE j is (CS0, c0) in s' -> CORE j is (CS0, c0) in s) /\
-      (forall n z z', CORE j is (CS0, c0) in s -> 
-                      safeN CS0 client_sig ge (S n) (s \o z) c0 m -> 
-                      safeN CS0 client_sig ge n (s' \o z') c0 m')))
-
-  (*if the extended machine is at external, then the active thread is at
-     external (an extension only implements external functions, it doesn't
-     introduce them)*)
-  (at_extern_call: forall s ef sig args,
-    at_external esem s = Some (ef, sig, args) -> 
-    exists CS, exists c, 
-      CORE (ACTIVE s) is (CS, c) in s /\ 
-      at_external CS c = Some (ef, sig, args))
-
-  (*inject the results of an external call into the extended machine state*)
-  (at_extern_ret: forall z s (c: cT (ACTIVE s)) m z' m' tys args ty ret c' CS ef sig x 
-      (P: ext_spec_type esig ef -> list typ -> list val -> Zext -> M -> Prop) 
-      (Q: ext_spec_type esig ef -> option typ -> option val -> Zext -> M -> Prop),
-    CORE (ACTIVE s) is (CS, c) in s -> 
-    at_external esem s = Some (ef, sig, args) -> 
-    spec_of ef esig = (P, Q) -> 
-    P x tys args (s \o z) m -> Q x ty ret z' m' -> 
-    after_external CS ret c = Some c' -> 
-    exists s': xT, 
-      z' = s' \o z' /\
-      after_external esem ret s = Some s' /\ 
-      CORE (ACTIVE s) is (CS, c') in s')
-
-  (*safety of other threads is preserved when returning from an external 
-     function call*)
-  (at_extern_rest: forall z s (c: cT (ACTIVE s)) m z' s' m' tys args ty ret c' CS ef x sig
-      (P: ext_spec_type esig ef -> list typ -> list val -> Zext -> M -> Prop) 
-      (Q: ext_spec_type esig ef -> option typ -> option val -> Zext -> M -> Prop),
-    CORE (ACTIVE s) is (CS, c) in s -> 
-    at_external esem s = Some (ef, sig, args) -> 
-    spec_of ef esig = (P, Q) -> 
-    P x tys args (s \o z) m -> Q x ty ret z' m' -> 
-    after_external CS ret c = Some c' -> 
-    after_external esem ret s = Some s' -> 
-    CORE (ACTIVE s) is (CS, c') in s' -> 
-    (forall j (CS0: CoreSemantics G (cT j) M D) c0, ACTIVE s <> j -> 
-      (CORE j is (CS0, c0) in s' -> CORE j is (CS0, c0) in s) /\
-      (forall ge n, CORE j is (CS0, c0) in s -> 
-                    safeN CS0 client_sig ge (S n) (s \o z) c0 m -> 
-                    safeN CS0 client_sig ge n (s' \o z') c0 m'))),
-  safety_criteria.
-
-Lemma safety_criteria_safe : safety_criteria -> safe_extension E.
+Program Definition ExtSound: EXTENSION_SOUNDNESS.Sig E.
 Proof.
+constructor.
 inversion 1; subst; intros ge n; induction n.
 intros s m z H1; simpl; auto.
 intros s m z H1.
@@ -401,14 +105,13 @@ rewrite H6 in H1; clear H6.
 destruct H1 as [x H1].
 destruct H1 as [H7 H8].
 generalize (Extension.esem_csem_linkable E); intros Hlink.
-assert (H16: IN ef (DIFF client_sig handled)).
+assert (H16: IN ef (DIFF csig handled)).
  apply in_diff.
- eapply Extension.at_external_client_sig; eauto.
- eapply Extension.at_external_not_handled; eauto.
- auto.
+ eapply Extension.at_external_csig; eauto.
+ solve[eapply Extension.at_external_not_handled with (esem := esem); eauto].
 specialize (Hlink ef 
   (ext_spec_pre esig ef) (ext_spec_post esig ef) 
-  (ext_spec_pre client_sig ef) (ext_spec_post client_sig ef) H16).
+  (ext_spec_pre csig ef) (ext_spec_post csig ef) H16).
 destruct Hlink with (x' := x) 
  (tys := sig_args sig) (args := args) (m := m) (z := (s \o z)) 
  as [x' [H17 H18]]; auto.
@@ -416,7 +119,6 @@ exists x'.
 erewrite at_external_not_handled; eauto.
 split; auto.
 rewrite Extension.zmult_proj in H17; auto.
-erewrite at_external_not_handled; eauto.
 intros ret m' z' POST.
 destruct (H8 ret m' (s \o z')) as [c' [H10 H11]].
 specialize (H18 (sig_res sig) ret m' (s \o z')).
@@ -465,7 +167,6 @@ destruct (at_extern_rest j CSj cj Hneq) as [H19 H20].
 rewrite <-H12.
 eapply H20; eauto.
 destruct H19 as [H21 H22]; auto.
-(*eapply H1'; eauto.*)
 
 (*CASE 2: at_external OUTER = None; i.e., inner corestep or handled function*)
 intros H2.
@@ -557,8 +258,8 @@ solve[destruct ef; elimtype False; auto].
 destruct H1 as [x H1].
 destruct H1 as [PRE POST].
 specialize (handled_pres ge s z m c0 s' m' cj CS ef sig args
-  (ext_spec_pre client_sig ef)
-  (ext_spec_post client_sig ef) x).
+  (ext_spec_pre csig ef)
+  (ext_spec_post csig ef) x).
 (*rewrite Heq in handled_pres.*)
 hnf in handled_pres.
 spec handled_pres; auto.
@@ -624,16 +325,16 @@ split; auto.
 rewrite H9 in PROJECT0; inversion PROJECT0; subst; auto.
 Qed.
 
-End SafetyCriteria.
+End ExtensionSoundness. End ExtensionSoundness.
 
 Section CoreCompat.
 Variables (G xT M D Z Zint Zext: Type) (cT: nat -> Type)
   (esem: CoreSemantics G xT M D) 
   (csem: forall i:nat, option (CoreSemantics G (cT i) M D))
-  (client_sig: ext_sig M Z)
+  (csig: ext_sig M Z)
   (esig: ext_sig M Zext)
   (handled: list AST.external_function)
-  (E: Extension.Sig cT Zint esem csem client_sig esig handled).
+  (E: Extension.Sig cT Zint esem csem csig esig handled).
 
 Import Extension.
 
@@ -792,9 +493,8 @@ Variables (fT: forall X:Type, Type) (cT dT D1 D2 Z Zint Zext: Type)
   (esem: forall (T: Type) (D: Type) (CS: CompcertCoreSem genv T D), 
     CompcertCoreSem genv (fT T) D) 
   (source: CompcertCoreSem genv cT D1) (target: CompcertCoreSem genv dT D2)
-  (client_sig: ext_sig mem Z) (esig: ext_sig mem Zext) (handled: list AST.external_function).
+  (csig: ext_sig mem Z) (esig: ext_sig mem Zext) (handled: list AST.external_function).
 
-Notation ALL_SAFE := (Extension.all_safe).
 Notation PROJ_CORE := (Extension.proj_core).
 Infix "\o" := (Extension.zmult) (at level 66, left associativity). 
 Notation ACTIVE := (Extension.active).
@@ -818,9 +518,9 @@ Definition cores (aT:Type) (D: Type) (CS: CompcertCoreSem genv aT D) :=
   fun i:nat => Some (csem CS).
 
 Variable (E1: Extension.Sig (fun _:nat => cT) Zint 
-  (esem source) (cores source) client_sig esig handled).
+  (esem source) (cores source) csig esig handled).
 Variable (E2: Extension.Sig (fun _:nat => dT) Zint 
-  (esem target) (cores target) client_sig esig handled).
+  (esem target) (cores target) csig esig handled).
 Variables (ge: genv) (entry_points: list (val*val*signature)).
 
 Import Sim_inj.
