veric/extension.v
@@ -1,0 +1,412 @@
+Load loadpath.
+Require Import msl.predicates_hered.
+Require Import veric.sim veric.step_lemmas veric.base veric.expr veric.extspec 
+               veric.juicy_extspec.
+Require Import ListSet.
+
+Set Implicit Arguments.
+
+(** External function specifications and linking *)
+
+Lemma extfunct_eqdec : forall ef1 ef2 : AST.external_function, 
+  {ef1=ef2} + {~ef1=ef2}.
+Proof. intros ef1 ef2; repeat decide equality; apply Address.EqDec_int. Qed.
+
+Module TruePropCoercion.
+Definition is_true (b: bool) := b=true.
+Coercion is_true: bool >-> Sortclass.
+End TruePropCoercion.
+
+Import TruePropCoercion.
+
+Notation IN := (ListSet.set_mem extfunct_eqdec).
+Notation NOTIN := (fun ef l => ListSet.set_mem extfunct_eqdec ef l = false).
+Notation DIFF := (ListSet.set_diff extfunct_eqdec).
+
+Lemma in_diff (ef: AST.external_function) (l r: list AST.external_function) :
+  IN ef l -> NOTIN ef r -> IN ef (DIFF l r).
+Proof.
+simpl; intros H1 H2; apply set_mem_correct2. 
+apply set_mem_correct1 in H1.
+apply set_mem_complete1 in H2.
+apply set_diff_intro; auto.
+Qed.
+
+(** Linking external specification [Sigma] with an extension implementing
+   functions in [handled] comprises removing the functions in [handled] from
+   the external specification. *)
+
+Definition link_ext_spec (M Z: Type) (handled: list AST.external_function) 
+  (Sigma: external_specification M AST.external_function Z) :=
+  Build_external_specification M AST.external_function Z
+    (ext_spec_type Sigma)
+    (fun (ef: AST.external_function) (x: ext_spec_type Sigma ef)
+         (tys: list typ) (args: list val) (z: Z) (m: M) => 
+             if ListSet.set_mem extfunct_eqdec ef handled then False 
+             else ext_spec_pre Sigma ef x tys args z m)
+    (fun (ef: AST.external_function) (x: ext_spec_type Sigma ef)
+         (ty: option typ) (ret: option val) (z: Z) (m: M) => 
+             if ListSet.set_mem extfunct_eqdec ef handled then True
+             else ext_spec_post Sigma ef x ty ret z m).
+
+Program Definition link_juicy_ext_spec (Z: Type) (handled: list AST.external_function)
+  (Sigma: juicy_ext_spec Z) :=
+  Build_juicy_ext_spec Z (link_ext_spec handled Sigma) _ _.
+Next Obligation.
+if_tac; [unfold hereditary; auto|].
+generalize JE_pre_hered; unfold hereditary; intros; eapply H; eauto.
+Qed.
+Next Obligation.
+if_tac; [unfold hereditary; auto|].
+generalize JE_post_hered; unfold hereditary; intros; eapply H; eauto.
+Qed.
+
+(** An external signature [ext_sig] is a list of handled functions together with
+   an external specification. *)
+
+Section ExtSig.
+Variables M Z: Type.
+
+Inductive ext_sig := 
+  mkextsig: forall (functs: list AST.external_function)
+                   (extspec: external_specification M external_function Z), 
+    ext_sig.
+
+Definition extsig2functs (Sigma: ext_sig) := 
+  match Sigma with mkextsig l _ => l end.
+Coercion extsig2functs : ext_sig >-> list.
+
+Definition extsig2extspec (Sigma: ext_sig) :=
+  match Sigma with mkextsig functs spec => spec end.
+Coercion extsig2extspec : ext_sig >-> external_specification.
+
+Definition spec_of (ef: AST.external_function) (Sigma: ext_sig) :=
+  (ext_spec_pre Sigma ef, ext_spec_post Sigma ef).
+
+End ExtSig.
+
+Record juicy_ext_sig (Z: Type): Type := mkjuicyextsig {
+  JE_functs:> list external_function;
+  JE_extspec:> juicy_ext_spec Z
+}.
+
+Definition juicy_extsig2extsig (Z: Type) (je: juicy_ext_sig Z) :=
+  mkextsig (JE_functs je) (JE_extspec je).
+Coercion juicy_extsig2extsig: juicy_ext_sig >-> ext_sig.
+
+Definition link (T Z: Type) (esig: ext_sig T Z) 
+      (handled: list AST.external_function) :=
+  mkextsig handled (link_ext_spec handled esig).
+
+Definition juicy_link (Z: Type) (jesig: juicy_ext_sig Z) 
+      (handled: list AST.external_function) :=
+  mkjuicyextsig handled (link_juicy_ext_spec handled jesig).
+
+(** A client signature is linkable with an extension signature when each
+   extension function specification ef:{P}{Q} is a subtype of the
+   specification ef:{P'}{Q'} assumed by client. *)
+
+Definition linkable (M Z Zext: Type) (proj_zext: Z -> Zext)
+      (handled: list AST.external_function) 
+      (csig: ext_sig M Z) (ext_sig: ext_sig M Zext) := 
+  forall ef P Q P' Q', 
+    IN ef (DIFF csig handled) -> 
+    spec_of ef ext_sig = (P, Q) -> 
+    spec_of ef csig = (P', Q') -> 
+    forall x' tys args m z, P' x' tys args z m -> 
+      exists x, P x tys args (proj_zext z) m /\
+      forall ty ret m' z', Q x ty ret (proj_zext z') m' -> Q' x' ty ret z' m'.
+
+(** * Extensions *)
+
+Module Extension. Section Extension.
+ Variables
+  (G: Type) (** global environments *)
+  (xT: Type) (** corestates of extended semantics *)
+  (cT: nat -> Type) (** corestates of core semantics *)
+  (M: Type) (** memories *)
+  (D: Type) (** initialization data *)
+  (Z: Type) (** external states *)
+  (Zint: Type) (** portion of Z implemented by extension *)
+  (Zext: Type) (** portion of Z external to extension *)
+
+  (esem: CoreSemantics G xT M D) (** extended semantics *)
+  (csem: forall i:nat, option (CoreSemantics G (cT i) M D)) (** a set of core semantics *)
+
+  (csig: ext_sig M Z) (** client signature *)
+  (esig: ext_sig M Zext) (** extension signature *)
+  (handled: list AST.external_function). (** functions handled by this extension *)
+
+ Record Sig := Make {
+ (** generalized projection of core [i] from state [s] *)
+   proj_core : forall i:nat, xT -> option (cT i);
+   core_exists : forall ge i s c' m s' m', 
+     corestep esem ge s m s' m' -> proj_core i s' = Some c' -> 
+     exists c, proj_core i s = Some c;
+   
+ (** the active (i.e., currently scheduled) core *)
+   active : xT -> nat;
+   active_csem : forall s, exists CS, csem (active s) = Some CS;
+   active_proj_core : forall s, exists c, proj_core (active s) s = Some c;
+   
+ (** Runnable=[true] when [active s] is runnable (i.e., not blocked
+    waiting on an external function call and not safely halted). *)
+   runnable : G -> xT -> bool;
+   runnable_false : forall ge s c CS,
+     runnable ge s = false -> 
+     csem (active s) = Some CS -> proj_core (active s) s = Some c -> 
+     (exists rv, safely_halted CS ge c = Some rv) \/
+     (exists ef, exists sig, exists args, at_external CS c = Some (ef, sig, args));
+
+ (** A core is no longer "at external" once the extension has returned 
+    to it with the result of the call on which it was blocked. *)
+   after_at_external_excl : forall i CS c c' ret,
+     csem i = Some CS -> after_external CS ret c = Some c' -> 
+     at_external CS c' = None;
+   
+   at_external_csig: forall s i CS c ef args sig,
+     csem i = Some CS -> proj_core i s = Some c -> 
+     at_external CS c = Some (ef, sig, args) -> 
+     IN ef csig;
+   notat_external_handled: forall s i CS c ef args sig,
+     csem i = Some CS -> proj_core i s = Some c -> 
+     at_external CS c = Some (ef, sig, args) -> 
+     at_external esem s = None -> 
+     IN ef handled;
+   at_external_not_handled: forall s ef args sig,
+     at_external esem s = Some (ef, sig, args) -> 
+     NOTIN ef handled;
+
+ (** Type [xT] embeds [Zint]. *)
+   proj_zint: xT -> Zint;
+   proj_zext: Z -> Zext;
+   zmult: Zint -> Zext -> Z;
+   zmult_proj: forall zint zext, proj_zext (zmult zint zext) = zext;
+
+ (** Implemented "external" state is unchanged after truly external calls. *)
+   ext_upd_at_external : forall ef sig args ret s s',
+     at_external esem s = Some (ef, sig, args) -> 
+     after_external esem ret s = Some s' -> 
+     proj_zint s = proj_zint s';
+   
+ (** [esem] and [csem] are signature linkable *)
+   esem_csem_linkable: linkable proj_zext handled csig esig
+ }.
+
+End Extension. End Extension.
+
+Implicit Arguments Extension.Make [G xT cT M D Z Zint Zext].
+
+(** * Safe Extensions *)
+
+Section AllSafety.
+ Variables
+  (G: Type) (** global environments *)
+  (xT: Type) (** corestates of extended semantics *)
+  (cT: nat -> Type) (** corestates of core semantics *)
+  (M: Type) (** memories *)
+  (D: Type) (** initialization data *)
+  (Z: Type) (** external states *)
+  (Zint: Type) (** portion of Z implemented by extension *)
+  (Zext: Type) (** portion of Z external to extension *)
+
+  (esem: CoreSemantics G xT M D) (** extended semantics *)
+  (csem: forall i:nat, option (CoreSemantics G (cT i) M D)) (** a set of core semantics *)
+
+  (csig: ext_sig M Z) (** client signature *)
+  (esig: ext_sig M Zext) (** extension signature *)
+  (handled: list AST.external_function). (** functions handled by this extension *)
+
+Import Extension.
+
+(** a global invariant characterizing "safe" extensions *)
+Definition all_safe (E: Sig cT Zint esem csem csig esig handled)
+  (ge: G) (n: nat) (z: Z) (w: xT) (m: M) :=
+     forall i CS c, csem i = Some CS -> proj_core E i w = Some c -> 
+       safeN CS csig ge n z c m.
+
+(** All-safety implies safeN. *)
+Definition safe_extension (E: Sig cT Zint esem csem csig esig handled) :=
+  forall ge n s m z, 
+    all_safe E ge n (zmult E (proj_zint E s) z) s m -> 
+    safeN esem (link esig handled) ge n z s m.
+
+End AllSafety.
+
+Module SafetyInterpolant. Section SafetyInterpolant.
+ Variables
+  (G: Type) (** global environments *)
+  (xT: Type) (** corestates of extended semantics *)
+  (cT: nat -> Type) (** corestates of core semantics *)
+  (M: Type) (** memories *)
+  (D: Type) (** initialization data *)
+  (Z: Type) (** external states *)
+  (Zint: Type) (** portion of Z implemented by extension *)
+  (Zext: Type) (** portion of Z external to extension *)
+
+  (esem: CoreSemantics G xT M D) (** extended semantics *)
+  (csem: forall i:nat, option (CoreSemantics G (cT i) M D)) (** a set of core semantics *)
+
+  (csig: ext_sig M Z) (** client signature *)
+  (esig: ext_sig M Zext) (** extension signature *)
+  (handled: list AST.external_function) (** functions handled by this extension *)
+  (E: Extension.Sig cT Zint esem csem csig esig handled). 
+
+Definition proj_zint := E.(Extension.proj_zint). 
+Coercion proj_zint : xT >-> Zint.
+
+Definition proj_zext := E.(Extension.proj_zext).
+Coercion proj_zext : Z >-> Zext.
+
+Notation ALL_SAFE := (all_safe E).
+Notation PROJ_CORE := E.(Extension.proj_core).
+Notation "zint \o zext" := (E.(Extension.zmult) zint zext) 
+  (at level 66, left associativity). 
+Notation ACTIVE := (E.(Extension.active)).
+Notation RUNNABLE := (E.(Extension.runnable)).
+Notation "'CORE' i 'is' ( CS , c ) 'in' s" := 
+  (csem i = Some CS /\ PROJ_CORE i s = Some c)
+  (at level 66, no associativity).
+Notation core_exists := E.(Extension.core_exists).
+Notation active_csem := E.(Extension.active_csem).
+Notation active_proj_core := E.(Extension.active_proj_core).
+Notation after_at_external_excl := E.(Extension.after_at_external_excl).
+Notation notat_external_handled := E.(Extension.notat_external_handled).
+Notation at_external_not_handled := E.(Extension.at_external_not_handled).
+Notation ext_upd_at_external := E.(Extension.ext_upd_at_external).
+Notation runnable_false := E.(Extension.runnable_false).
+
+Inductive safety_interpolant: Type := SafetyInterpolant: forall 
+  (** Coresteps preserve the all-safety invariant. *)
+  (core_pres: forall ge n z (s: xT) c m CS s' c' m', 
+    ALL_SAFE ge (S n) (s \o z) s m -> 
+    CORE (ACTIVE s) is (CS, c) in s -> 
+    corestep CS ge c m c' m' -> corestep esem ge s m s' m' -> 
+    ALL_SAFE ge n (s' \o z) s' m')
+
+  (** Corestates satisfying the invariant can corestep. *)
+  (core_prog: forall ge n z s m c CS, 
+    ALL_SAFE ge (S n) z s m -> 
+    RUNNABLE ge s=true -> CORE (ACTIVE s) is (CS, c) in s -> 
+    exists c', exists s', exists m', 
+      corestep CS ge c m c' m' /\ corestep esem ge s m s' m' /\
+      CORE (ACTIVE s) is (CS, c') in s')
+
+  (** "Handled" steps respect function specifications. *)
+  (handled_pres: forall ge s z m (c: cT (ACTIVE s)) s' m' (c': cT (ACTIVE s)) 
+      (CS: CoreSemantics G (cT (ACTIVE s)) M D) ef sig args P Q x, 
+    let i := ACTIVE s in CORE i is (CS, c) in s -> 
+    at_external CS c = Some (ef, sig, args) -> 
+    ListSet.set_mem extfunct_eqdec ef handled = true -> 
+    spec_of ef csig = (P, Q) -> 
+    P x (sig_args sig) args (s \o z) m -> 
+    corestep esem ge s m s' m' -> 
+    CORE i is (CS, c') in s' -> 
+      ((at_external CS c' = Some (ef, sig, args) /\ P x (sig_args sig) args (s' \o z) m' /\
+        (forall j, ACTIVE s' = j -> i <> j)) \/
+      (exists ret, after_external CS ret c = Some c' /\ Q x (sig_res sig) ret (s' \o z) m')))
+
+  (** "Handled" states satisfying the invariant can step or are safely halted;
+     core states that remain "at_external" over handled steps are unchanged. *)
+  (handled_prog: forall ge n (z: Zext) (s: xT) m,
+    ALL_SAFE ge (S n) (s \o z) s m -> 
+    RUNNABLE ge s=false -> 
+    at_external esem s = None -> 
+    (exists s', exists m', corestep esem ge s m s' m' /\ 
+      forall i c CS, CORE i is (CS, c) in s -> 
+        exists c', CORE i is (CS, c') in s' /\ 
+          (forall ef args ef' args', 
+            at_external CS c = Some (ef, args) -> 
+            at_external CS c' = Some (ef', args') -> c=c')) \/
+    (exists rv, safely_halted esem ge s = Some rv))
+
+  (** Safely halted threads remain halted. *)
+  (safely_halted_halted: forall ge s m s' m' i CS c rv,
+    CORE i is (CS, c) in s -> 
+    safely_halted CS ge c = Some rv -> 
+    corestep esem ge s m s' m' -> 
+    CORE i is (CS, c) in s')
+
+  (** Safety of other threads is preserved when handling one step of blocked
+     thread [i]. *)
+  (handled_rest: forall ge s m s' m' c CS,
+    CORE (ACTIVE s) is (CS, c) in s -> 
+    ((exists ef, exists sig, exists args, at_external CS c = Some (ef, sig, args)) \/ 
+      exists rv, safely_halted CS ge c = Some rv) -> 
+    at_external esem s = None -> 
+    corestep esem ge s m s' m' -> 
+    (forall j (CS0: CoreSemantics G (cT j) M D) c0, ACTIVE s <> j ->  
+      (CORE j is (CS0, c0) in s' -> CORE j is (CS0, c0) in s) /\
+      (forall n z z', CORE j is (CS0, c0) in s -> 
+                      safeN CS0 csig ge (S n) (s \o z) c0 m -> 
+                      safeN CS0 csig ge n (s' \o z') c0 m')))
+
+  (** If the extended machine is at external, then the active thread is at
+     external (an extension only implements external functions, it doesn't
+     introduce them). *)
+  (at_extern_call: forall s ef sig args,
+    at_external esem s = Some (ef, sig, args) -> 
+    exists CS, exists c, 
+      CORE (ACTIVE s) is (CS, c) in s /\ 
+      at_external CS c = Some (ef, sig, args))
+
+  (** Inject the results of an external call into the extended machine state. *)
+  (at_extern_ret: forall z s (c: cT (ACTIVE s)) m z' m' tys args ty ret c' CS ef sig x 
+      (P: ext_spec_type esig ef -> list typ -> list val -> Zext -> M -> Prop) 
+      (Q: ext_spec_type esig ef -> option typ -> option val -> Zext -> M -> Prop),
+    CORE (ACTIVE s) is (CS, c) in s -> 
+    at_external esem s = Some (ef, sig, args) -> 
+    spec_of ef esig = (P, Q) -> 
+    P x tys args (s \o z) m -> Q x ty ret z' m' -> 
+    after_external CS ret c = Some c' -> 
+    exists s': xT, 
+      z' = s' \o z' /\
+      after_external esem ret s = Some s' /\ 
+      CORE (ACTIVE s) is (CS, c') in s')
+
+  (** Safety of other threads is preserved when returning from an external 
+     function call. *)
+  (at_extern_rest: forall z s (c: cT (ACTIVE s)) m z' s' m' tys args ty ret c' CS ef x sig
+      (P: ext_spec_type esig ef -> list typ -> list val -> Zext -> M -> Prop) 
+      (Q: ext_spec_type esig ef -> option typ -> option val -> Zext -> M -> Prop),
+    CORE (ACTIVE s) is (CS, c) in s -> 
+    at_external esem s = Some (ef, sig, args) -> 
+    spec_of ef esig = (P, Q) -> 
+    P x tys args (s \o z) m -> Q x ty ret z' m' -> 
+    after_external CS ret c = Some c' -> 
+    after_external esem ret s = Some s' -> 
+    CORE (ACTIVE s) is (CS, c') in s' -> 
+    (forall j (CS0: CoreSemantics G (cT j) M D) c0, ACTIVE s <> j -> 
+      (CORE j is (CS0, c0) in s' -> CORE j is (CS0, c0) in s) /\
+      (forall ge n, CORE j is (CS0, c0) in s -> 
+                    safeN CS0 csig ge (S n) (s \o z) c0 m -> 
+                    safeN CS0 csig ge n (s' \o z') c0 m'))),
+  safety_interpolant.
+
+End SafetyInterpolant. End SafetyInterpolant.
+
+Module EXTENSION_SOUNDNESS. Section EXTENSION_SOUNDNESS.
+ Variables
+  (G: Type) (** global environments *)
+  (xT: Type) (** corestates of extended semantics *)
+  (cT: nat -> Type) (** corestates of core semantics *)
+  (M: Type) (** memories *)
+  (D: Type) (** initialization data *)
+  (Z: Type) (** external states *)
+  (Zint: Type) (** portion of Z implemented by extension *)
+  (Zext: Type) (** portion of Z external to extension *)
+
+  (esem: CoreSemantics G xT M D) (** extended semantics *)
+  (csem: forall i:nat, option (CoreSemantics G (cT i) M D)) (** a set of core semantics *)
+
+  (csig: ext_sig M Z) (** client signature *)
+  (esig: ext_sig M Zext) (** extension signature *)
+  (handled: list AST.external_function) (** functions handled by this extension *)
+  (E: Extension.Sig cT Zint esem csem csig esig handled). 
+
+Import SafetyInterpolant.
+
+Record Sig := Make {extension_sound: safety_interpolant E -> safe_extension E}.
+
+End EXTENSION_SOUNDNESS. End EXTENSION_SOUNDNESS.
+
