veric/seplog_extension.v
@@ -1,7 +1,7 @@
 Load loadpath.
 Require Import msl.ageable msl.rmaps.
 Require Import veric.sim veric.step_lemmas veric.base veric.expr 
-               veric.extspec veric.extensions veric.juicy_extspec veric.compcert_rmaps
+               veric.extspec veric.extension veric.juicy_extspec veric.compcert_rmaps
                veric.semax veric.SeparationLogic veric.SeparationLogicSoundness.
 Import juicy_mem.
 
@@ -15,55 +15,59 @@ Fixpoint externals (fs: list (ident*fundef)) :=
   end.
 
 Module SEPLOG_EXTENSION_SOUNDNESS (EXT_SPEC: EXTERNAL_SPEC). Import EXT_SPEC.
-Module SepLog := MakeSeparationLogic EXT_SPEC. Import SepLog.
-Section seplog_extension_soundness. Variable (prog: program).
 
-Definition juicy_client_sig: juicy_ext_sig Z :=
-  mkjuicyextsig (externals (prog_funct prog)) Hspec.
+Module SepLog := MakeSeparationLogic(EXT_SPEC). Import SepLog.
 
-Variables (juicy_esig: juicy_ext_sig Z)
-  (Hlinkable: linkable (externals (prog_funct prog)) juicy_client_sig juicy_esig).
+Section SeplogExtensionSoundness. 
+Variable prog: program.
+ Variables
+  (xT: Type) (** corestates of extended semantics *)
+  (Zint: Type) (** portion of Z implemented by extension *)
+  (Zext: Type). (** portion of Z external to extension *)
+
+Definition juicy_csig: juicy_ext_sig Z :=
+  mkjuicyextsig (externals (prog_funct prog)) CSL.ExtSpec.Hspec.
 
 Definition initial_cores (i: nat) := 
   if eq_nat_dec i 1 then Some (juicy_core_sem Clight_new.cl_core_sem)
   else None.
 
-(*the following restrictions on the extension definition may need to be nuanced a bit*)
-Let gT := Genv.t fundef type.
-Variables (xT Zint Zext: Type).
-Variable (ext_coresem: CoreSemantics gT xT juicy_mem jm_init_package).
-
-Variable (ext: Extension.Sig Zint Zext ext_coresem initial_cores 
-                 juicy_client_sig juicy_esig (externals (prog_funct prog))).
-Variable (Hsafe: safe_extension ext).
-Variable (Hinit: forall b q0, 
+ Variables
+  (esem: CoreSemantics (Genv.t fundef type) xT juicy_mem jm_init_package) (** extended semantics *)
+  (juicy_esig: juicy_ext_sig Z)
+  (handled: list AST.external_function) (** functions handled by this extension *)
+  (E: Extension.Sig (fun _:nat => Clight_new.corestate) Zint esem initial_cores 
+    juicy_csig juicy_esig (externals (prog_funct prog)))
+  (Hlinkable: linkable (Extension.proj_zext E) (externals (prog_funct prog)) 
+    juicy_csig juicy_esig)
+ (Hsafe: safe_extension E)
+ (Hinit: forall b q0, 
   Genv.find_symbol (Genv.globalenv prog) (prog_main prog) = Some b -> 
   make_initial_core (juicy_core_sem Clight_new.cl_core_sem) (Genv.globalenv prog) 
           (Vptr b Int.zero) nil = Some q0 -> 
-  exists q, make_initial_core ext_coresem (Genv.globalenv prog) 
+  exists q, make_initial_core esem (Genv.globalenv prog) 
           (Vptr b Int.zero) nil = Some q /\
-    Extension.proj_core ext q 1 = Some q0).
+    Extension.proj_core E 1 q = Some q0).
 
-Theorem semax_extension_rule (z: Z) (G: funspecs) (m: mem) :
-  CSL.semax_prog prog G -> 
+Lemma semax_extension_rule (z: Z) (V: varspecs) (G: funspecs) (m: mem):
+  CSL.semax_prog prog V G -> 
   Genv.init_mem prog = Some m -> 
   exists b: block, exists q: xT,
     Genv.find_symbol (Genv.globalenv prog) (prog_main prog) = Some b /\
-    make_initial_core ext_coresem (Genv.globalenv prog) (Vptr b Int.zero) nil = Some q /\
+    make_initial_core esem (Genv.globalenv prog) (Vptr b Int.zero) nil = Some q /\
     (forall n: nat,
       exists jm : juicy_mem.juicy_mem,
         juicy_mem.m_dry jm = m /\
         ageable.level jm = n /\
-        safeN ext_coresem (juicy_link juicy_esig (externals (prog_funct prog))) 
-            (Genv.globalenv prog) n (Extension.zmult ext (Extension.proj_zint ext q) 
-               (Extension.proj_zext ext z)) q jm).
+        safeN esem (juicy_link juicy_esig (externals (prog_funct prog))) 
+            (Genv.globalenv prog) n (Extension.proj_zext E z) q jm).
 Proof.
 intros H1 H2.
-destruct (semax_prog_rule z G prog m H1 H2) as [b [q0 [H3 [H4 H5]]]].
+destruct (semax_prog_rule z V G prog m H1 H2) as [b [q0 [H3 [H4 H5]]]].
 destruct (Hinit H3 H4) as [q [H6 H7]].
 destruct (semax_prog_rule 
-  (Extension.zmult ext (Extension.proj_zint ext q) (Extension.proj_zext ext z)) 
-  G prog m H1 H2) 
+  (Extension.zmult E (Extension.proj_zint E q) (Extension.proj_zext E z)) 
+  V G prog m H1 H2) 
  as [b' [q0' [H3' [H4' H5']]]].
 rewrite H3 in H3'; inv H3'.
 rewrite H4 in H4'; inv H4'.
@@ -75,7 +79,7 @@ simpl.
 simpl in Hsafe.
 specialize (@Hsafe (Genv.globalenv prog) (@ageable.level _ ag_rmap (m_phi jm)) q jm).
 eapply Hsafe.
-unfold Extension.all_safe.
+unfold all_safe.
 unfold initial_cores.
 intros i ? ?.
 if_tac; subst.
@@ -87,6 +91,6 @@ apply H10.
 inversion 1.
 Qed.
 
-End seplog_extension_soundness. 
-End SEPLOG_EXTENSION_SOUNDNESS.
+End SeplogExtensionSoundness.
 
+End SEPLOG_EXTENSION_SOUNDNESS.
